Coq/src/drf/Race.v
@@ -1,13 +1,15 @@
 From hahn Require Import Hahn.
 From imm Require Import Events Prog RC11.
+Require Import SC.
+
 Require Import AuxRel.
 Require Import EventStructure.
 Require Import Consistency.
 Require Import Execution.
 Require Import ExecutionToG.
+Require Import Step.
+Require Import ProgES.
 
-Module Race.
-  
 Section Race.
 
 Variable S : ES.t.
@@ -27,22 +29,33 @@ Notation "'Rel'" := (fun a => is_true (is_rel S.(ES.lab) a)) (at level 10).
 Notation "'Acq'" := (fun a => is_true (is_acq S.(ES.lab) a)) (at level 10).
 Notation "'Sc'" := (fun a => is_true (is_sc S.(ES.lab) a)) (at level 10).
 
-Definition one {A : Type} (X : A -> Prop) a b := X a \/ X b. 
+Definition one {A : Type} (X : A -> Prop) a b := X a \/ X b.
 
 Definition race (X : eventid -> Prop) :=
   dom_rel ((X × X) \ (hb⁼ ∪ cf) ∩ same_loc ∩ one W). (* hb should be hbc11? *)
 
 Definition RLX_race_free (X : eventid -> Prop) :=
-  race X ⊆₁ (Rel ∩₁ W) ∪₁ (Acq ∩₁ R). 
+  race X ⊆₁ (Rel ∩₁ W) ∪₁ (Acq ∩₁ R).
 
 Definition rc11_consistent_x (S : ES.t) (X : eventid -> Prop) := exists G,
     ⟪ x2g  : X2G S X G ⟫ /\
-    ⟪ rc11 : rc11_consistent G ⟫.  
+    ⟪ rc11 : rc11_consistent G ⟫.
 
 Definition RA_race_free (X : eventid -> Prop) :=
   race X ⊆₁ Sc.
 
+Definition sc_consistent_x (S : ES.t) (X : eventid -> Prop) := exists G,
+    ⟪ x2g  : X2G S X G ⟫ /\
+    ⟪ sc : sc_consistent G ⟫.
 
 End Race.
 
-End Race.
+Definition program_execution P S X :=
+  ⟪ STEPS : (step Weakestmo)＊ (prog_es_init P) S⟫ /\
+  ⟪ EXEC : Execution.t S X ⟫.
+
+Definition RC11_RLX_race_free_program P :=
+  (forall S X, program_execution P S X -> rc11_consistent_x S X -> RLX_race_free S X).
+
+Definition SC_RA_race_free_program P :=
+  (forall S X, program_execution P S X -> sc_consistent_x S X -> RA_race_free S X).
