Coq/src/drf/DRF_WEAKESTMO_SC.v
@@ -1,0 +1,58 @@
+From hahn Require Import Hahn.
+From imm Require Import Events Prog ProgToExecutionProperties RC11.
+From PromisingLib Require Import Basic.
+Require Import AuxDef.
+Require Import AuxRel.
+Require Import EventStructure.
+Require Import Consistency.
+Require Import Execution.
+Require Import Step.
+Require Import Race.
+Require Import ProgES.
+Require Import StepWf.
+Require Import ExecutionToG.
+
+Set Implicit Arguments.
+
+Module DRF_WEAKESTMO_SC.
+
+Notation "'E' S" := S.(ES.acts_set) (at level 10).
+Notation "'Einit' S"  := S.(ES.acts_init_set) (at level 10).
+Notation "'Eninit' S" := S.(ES.acts_ninit_set) (at level 10).
+
+Notation "'tid' S" := S.(ES.tid) (at level 10).
+Notation "'lab' S" := S.(ES.lab) (at level 10).
+Notation "'mod' S" := (Events.mod S.(ES.lab)) (at level 10).
+Notation "'loc' S" := (Events.loc S.(ES.lab)) (at level 10).
+Notation "'val' S" := (Events.val S.(ES.lab)) (at level 10).
+
+Notation "'sb' S" := S.(ES.sb) (at level 10).
+Notation "'rmw' S" := S.(ES.rmw) (at level 10).
+Notation "'ew' S" := S.(ES.ew) (at level 10).
+Notation "'jf' S" := S.(ES.jf) (at level 10).
+Notation "'rf' S" := S.(ES.rf) (at level 10).
+Notation "'co' S" := S.(ES.co) (at level 10).
+Notation "'cf' S" := S.(ES.cf) (at level 10).
+
+Notation "'jfe' S" := S.(ES.jfe) (at level 10).
+Notation "'rfe' S" := S.(ES.rfe) (at level 10).
+Notation "'coe' S" := S.(ES.coe) (at level 10).
+Notation "'jfi' S" := S.(ES.jfi) (at level 10).
+Notation "'rfi' S" := S.(ES.rfi) (at level 10).
+Notation "'coi' S" := S.(ES.coi) (at level 10).
+
+Notation "'R' S" := (fun a => is_true (is_r S.(ES.lab) a)) (at level 10).
+Notation "'W' S" := (fun a => is_true (is_w S.(ES.lab) a)) (at level 10).
+Notation "'F' S" := (fun a => is_true (is_f S.(ES.lab) a)) (at level 10).
+
+Notation "'Rel' S" := (fun a => is_true (is_rel S.(ES.lab) a)) (at level 10).
+Notation "'Acq' S" := (fun a => is_true (is_acq S.(ES.lab) a)) (at level 10).
+
+Theorem DRF_WEAKESTMO_SC P S X
+      (RA_RACE_FREE : SC_RA_race_free_program P)
+      (EXEC : program_execution P S X) :
+  sc_consistent_x S X.
+Proof.
+Admitted.
+
+End DRF_WEAKESTMO_SC.
